## Introduction to Differential Equations and their Solutions

**Conceptual Difference from Algebraic Equations**

In algebraic equations such as x^2 + 1 = 0 or sin^2 x - cos x = 0, solutions are numbers (real or complex) that satisfy the given equations by substituting the unknown variable. However, in differential equations, the unknown is a function rather than a single value. Specifically, the solution is a function y = Ï†(x) such that when substituted into the differential equation along with its derivatives, it satisfies the equality. This represents a fundamental shift from finding a number that satisfies an equation to finding a function that satisfies a relation involving derivatives.



## General Solution versus Particular Solution

**General Solution of a Differential Equation**

The general solution of a differential equation is a family of functions that contain arbitrary constants (often denoted as parameters such as a and b). These constants allow the general solution to represent all possible solutions of the differential equation. For example, for the differential equation \(\frac{d^2 y}{dx^2} + y = 0\), the function \(y = a\sin(x + b)\) where a and b are arbitrary real constants, is a general solution. This encapsulates infinitely many solution curves, each corresponding to particular values of a and b.

**Particular Solution of a Differential Equation**

A particular solution is derived from the general solution by assigning specific values to the arbitrary constants. This procedure yields a unique solution curve that satisfies the differential equation for the given constants. For instance, assigning \(a=2\) and \(b=\frac{\pi}{4}\) to the general solution \(y = a\sin(x + b)\) results in a particular solution \(y = 2\sin\left(x + \frac{\pi}{4}\right)\). Particular solutions are useful when initial or boundary conditions are specified.



## Verification of Solutions with Examples

**Example 1: Verifying \(y = e^{-3x}\) as Solution**

Given the differential equation \(\frac{d^2 y}{dx^2} + 2\frac{dy}{dx} - 6y = 0\), we verify that \(y = e^{-3x}\) solves it. First, calculate derivatives: \(\frac{dy}{dx} = -3 e^{-3x}\) and \(\frac{d^2 y}{dx^2} = 9 e^{-3x}\). Substitute into the differential equation's left-hand side (LHS): \(9 e^{-3x} + 2(-3 e^{-3x}) - 6 e^{-3x} = 9 e^{-3x} - 6 e^{-3x} - 6 e^{-3x} = 0\), which equals the right-hand side, confirming \(y = e^{-3x}\) is a solution.

**Example 2: Verifying \(y = a \cos x + b \sin x\) as Solution**

For the differential equation \(\frac{d^2 y}{dx^2} + y = 0\), consider \(y = a \cos x + b \sin x\) where a and b are real constants. Differentiating twice yields \(\frac{dy}{dx} = -a \sin x + b \cos x\) and \(\frac{d^2 y}{dx^2} = -a \cos x - b \sin x\). Substituting back into the left side gives: \((-a \cos x - b \sin x) + (a \cos x + b \sin x) = 0\), satisfying the differential equation. This demonstrates that the given function with arbitrary constants is indeed a general solution.


