## Definition and Form of First Order Linear Differential Equations

**Standard Form**

A first order linear differential equation is any differential equation that can be expressed in the form \( \frac{dy}{dx} + P(x)y = Q(x) \) where \(P(x)\) and \(Q(x)\) are given functions of the independent variable \(x\), or constants. This form is central because it allows a systematic method of solution via integrating factors. This form is linear in the unknown function \(y\) and its derivative \(dy/dx\).

**Alternative Form**

There exists an alternative formulation of first order linear differential equations where \(x\) is considered dependent and \(y\) independent, written as \( \frac{dx}{dy} + P_1(y)x = Q_1(y) \). Here, \(P_1(y)\) and \(Q_1(y)\) are functions of the variable \(y\) alone or constants. This form can be treated analogously by finding an integrating factor relative to \(y\).



## Integrating Factor (I.F.)

**Purpose and Definition**

The integrating factor is a function of \(x\), denoted \(g(x)\), chosen to multiply the entire differential equation so that the left hand side becomes the total derivative of \(y\times g(x)\) with respect to \(x\). This enables direct integration. The integrating factor is given by \(g(x) = e^{\int P(x) dx}\). This exponential construction ensures that \( \frac{d}{dx}[y g(x)] = g(x) \frac{dy}{dx} + y g'(x) \) matches the original equationâ€™s left side.

**Derivation**

Starting from \( \frac{dy}{dx} + P(x) y = Q(x) \), multiply both sides by a function \(g(x)\), to get \( g(x) \frac{dy}{dx} + P(x) g(x) y = Q(x) g(x)\). If \(g(x)\) is chosen such that \( \frac{d}{dx} [y g(x)] = g(x) \frac{dy}{dx} + y g'(x) = g(x) \frac{dy}{dx} + P(x) g(x) y \), then it must be \(g'(x) = P(x) g(x)\). Solving this gives \( g(x) = e^{\int P(x) dx} \). This ensures left side is \( \frac{d}{dx}[y g(x)] \).

**Using Integrating Factor**

Multiply the entire differential equation by the integrating factor. This transforms the differential equation into \( \frac{d}{dx}[y \, g(x)] = Q(x) g(x) \). Integrate both sides with respect to \(x\), yielding \( y \, g(x) = \int Q(x) g(x) \, dx + C \). Solving for \(y\) gives the general solution.



## Step-by-Step Solution Procedure

**Step 1**

Write the given differential equation explicitly in the linear form: \( \frac{dy}{dx} + P(x) y = Q(x) \). Identify functions or constants \(P\) and \(Q\).

**Step 2**

Compute the integrating factor \(I.F. = e^{\int P(x) dx} \). This is essential to transforming the equation into an integrable form.

**Step 3**

Multiply the entire differential equation by the integrating factor \(I.F.\), converting the left side into the derivative of the product \(y \times I.F.\).

**Step 4**

Integrate both sides of the resulting equation with respect to \(x\): \( \int \frac{d}{dx} [y \times I.F.] dx = \int Q(x) \times I.F. \, dx \) giving \( y \times I.F. = \int Q(x) \times I.F. \, dx + C \).

**Step 5**

Finally, solve for \(y\) by dividing by the integrating factor: \( y = \frac{1}{I.F.} \left[ \int Q(x) \times I.F. \, dx + C \right] \). This expression represents the general solution.



## Handling the Alternative Form dy/dx + P1(y)x = Q1(y)

**Integrating Factor**

For the differential equation of the form \( \frac{dx}{dy} + P_1(y) x = Q_1(y) \), the integrating factor is computed with respect to \(y\) as \( I.F. = e^{\int P_1(y) dy} \). This converts the left hand side into \( \frac{d}{dy}[x \times I.F.] \).

**General Solution**

Multiplying the differential equation by the integrating factor, then integrating both sides with respect to \(y\) yields \( x \times I.F. = \int Q_1(y) \times I.F. \, dy + C \), and then solving for \(x\) provides the solution.



## Examples

**Example 14: Solve \( \frac{dy}{dx} - y = \cos x \)**

Rewrite as \( \frac{dy}{dx} + (-1) y = \cos x \) with \(P = -1\), \(Q = \cos x\). Integrating Factor: \(I.F. = e^{\int -1 dx} = e^{-x}\). Multiply entire equation by \( e^{-x} \) to get \( \frac{d}{dx}[y e^{-x}] = e^{-x} \cos x \). Integrate the right side using integration by parts and algebraic manipulation, resulting in \( \int e^{-x} \cos x dx = \frac{e^{-x}}{2} (\sin x - \cos x) + C \). Hence, \( y e^{-x} = \frac{e^{-x}}{2} (\sin x - \cos x) + C \), so \( y = \frac{\sin x - \cos x}{2} + C e^{x} \) is the general solution.

**Example 15: Solve \( \frac{dy}{dx} \cdot \frac{1}{x} + 2 y = x^2, x \neq 0 \)**

Rewrite as \( \frac{dy}{dx} + 2x y = x^3 \) after multiplying both sides by \(x\). Here, \(P = 2x\), \(Q = x^3\). Compute Integrating Factor: \(I.F. = e^{\int 2x dx} = e^{x^2} \). Multiply whole equation by \( e^{x^2} \), convert left side into derivative \( \frac{d}{dx} [y e^{x^2}] = x^3 e^{x^2} \). Integrate right side and simplify, then solve for \(y\). The integral \( \int x^3 e^{x^2} dx \) reduces via substitution; the final solution is given as \( y = \frac{x}{2} + C e^{-x^2} \).

**Example 16: Solve \( y dx - (x + 2 y^2) dy = 0 \)**

Rewrite as \( \frac{dx}{dy} - \frac{x}{y} = 2 y \). Identify \( P_1(y) = - \frac{1}{y} \) and \( Q_1(y) = 2 y \). Compute Integrating Factor: \( I.F. = e^{\int -1/y dy} = e^{-\ln y} = y^{-1} \). Multiply entire equation to obtain form \( \frac{d}{dy}[x y^{-1}] = 2 y \cdot y^{-1} = 2 \). Integrate \( \int 2 dy = 2y + C \), solve for \(x\): \( x y^{-1} = 2 y + C \), thus \( x = 2 y^{2} + C y \).

**Example 17: Solve \( \frac{dy}{dx} + y \cot x = 2x + x^{2} \cot x, x \neq 0 \) with \( y = 0 \) when \( x = \frac{\pi}{2} \)**

Identify \( P = \cot x \) and \( Q = 2x + x^{2} \cot x \). The integrating factor is \( I.F. = e^{\int \cot x dx} = e^{\ln |\sin x|} = \sin x \). Multiplying throughout, \( \frac{d}{dx}[y \sin x] = (2x + x^2 \cot x) \sin x = 2x \sin x + x^2 \cos x \). Integrate the right hand side using integration by parts and simplification to get \( y \sin x = x^{2} \sin x + C \). Apply boundary condition to find \( C = -\frac{\pi^{2}}{4} \), thus \( y = x^{2} - \frac{\pi^{2}}{4 \sin x} \) is the particular solution.

**Example 18: Find curve where slope of tangent at \((x,y)\) is \( x + x y \), passing through \((0,1)\)**

Given slope \( \frac{dy}{dx} = x + x y \), rewrite as \( \frac{dy}{dx} - x y = x \). Here, \( P = -x \), \( Q = x \). The integrating factor is \( I.F. = e^{\int -x dx} = e^{-\frac{x^{2}}{2}} \). Multiply equation by I.F.: \( \frac{d}{dx}[ y e^{-x^{2}/2} ] = x e^{-x^{2}/2} \). Use substitution to integrate right side, lifting solution to \( y e^{-x^{2}/2} = - e^{-x^{2}/2} + C \), or \( y = -1 + C e^{x^{2}/2} \). Use initial condition \( y(0) = 1 \) to find \( C = 2 \), giving final curve equation \( y = -1 + 2 e^{x^{2}/2} \).


